PA/draft.v
@@ -1,15 +1,4 @@
-tree_rec :
-	forall (A : Type) (P : tree A -> Set),
-    (forall (a : A) (f : forest A), P (node A a f)) ->
-    forall t : tree A, P t
-
-tree_forest_rec :
-	forall (A : Type) (P : tree A -> Set) (Q : forest A -> Set),
-    (forall (a : A) (f : forest A),
-	   Q f ->
-	   P (node A a f)) ->
-       Q (nil A) ->
-       (forall t : tree A,
-        P t -> forall f1 : forest A, Q f1 -> Q (next A t f1)) ->
-       forall t : tree A, P t
-
+Lemma EMF (A : Prop) : A \/ ~ A -> False.
+Proof.
+    intro.
+    
