PA/tp1.v
@@ -1,0 +1,224 @@
+Require Import Arith.
+
+Axiom todo : forall A, A.
+Ltac todo := apply todo.
+
+Goal True.
+  exact I.
+Qed.
+
+Check True.
+
+Print Module Init.Nat.
+
+Parameter A B C : Prop.
+
+Lemma AimpA : A -> A.
+Proof.
+  intro.
+  assumption.
+Qed.
+
+Lemma imp_trans : (A -> B) -> (B -> C) -> A -> C.
+Proof.
+  intros.
+  apply H0.
+  apply H.
+  assumption.
+Qed.
+
+Lemma and_comm : A /\ B -> B /\ A.
+Proof.
+  intro.
+  destruct H.
+  split; assumption.
+Qed.
+
+Lemma or_comm : A \/ B -> B \/ A.
+Proof.
+  intro.
+  destruct H; [right | left]; assumption.
+Qed.
+
+Lemma A_imp_nnA : A -> ~~A.
+Proof.
+  unfold not.  
+  intros.
+  apply H0.
+  assumption.
+Qed.
+
+Lemma distr_and_or : (A\/B)/\C -> A/\C \/ B/\C.
+Proof.
+  intros.
+  destruct H. 
+  destruct H. 
+  + left. split; assumption.
+  + right. split; assumption.
+Qed.
+
+Lemma equiv_refl : A <-> A.
+Proof.
+  unfold iff.
+  split; intro; assumption.
+Qed.
+
+(** 2.2 Classical logic *)
+
+Lemma equiv_classic :
+  (forall P, P \/ ~P) <-> (forall P, ~~P -> P).
+Proof.
+  unfold iff. 
+  split; unfold not; intros.  
+  - destruct H with P. 
+    + assumption.
+    + apply H0 in H1. contradiction.
+  - apply H.
+    intro.
+    apply H0.
+    right.
+    intro.
+    destruct H0; left; assumption.
+Qed.
+
+(* 2.2.1 {Classical formulae in an intuitionistic world *)
+(* Modelization of a definition and lemmas *)
+
+Definition is_classical (P:Prop) := ~~P -> P. 
+
+Lemma nn_funct (P Q : Prop) : ~~ P /\ (P -> Q) -> ~~Q.
+Proof.
+  unfold not.  
+  intro.
+  
+  destruct H.
+  intro. 
+  apply H1.
+  apply H0. 
+  destruct H.
+  intro.
+  apply H1.
+  apply H0.
+  assumption.
+Qed.
+
+Lemma class_t : is_classical True.
+Proof.
+  unfold is_classical.
+  unfold not.
+  intro.
+  trivial.
+Qed.
+  
+Lemma class_f : is_classical False.
+Proof.
+  unfold is_classical.
+  unfold not.
+  intro.
+  destruct H.
+  intro.
+  assumption.
+Qed.
+
+Lemma class_conj (P Q : Prop) : is_classical P /\ is_classical Q -> is_classical (P /\ Q).
+Proof.
+  unfold is_classical.
+  unfold not.
+  intro.
+  destruct H.
+  intro.
+  split.
+  - apply H.
+    intro.
+    apply H1.
+    intro.
+    destruct H3. apply H2. apply H3.
+  - apply H0.
+    intro.
+    apply H1.
+    intro.
+    destruct H3. apply H2. apply H4.
+Qed.  
+
+
+
+(* 3.1 Socrates *)
+(* Modelization using axioms *)
+Parameter Person:Type.
+Parameter Socrate : Person.
+Parameter Men Mortal : Person->Prop.
+
+Lemma socrateMortal : Men Socrate /\ (forall P:Person, Men P -> Mortal P) -> Mortal Socrate.
+Proof.
+  intro.
+  destruct H.
+  apply H0 in H.
+  assumption.
+Qed.
+
+
+(* 3.2 Drinkers paradox *)
+(* Modelization using axioms + classical logic *)
+Parameter EM : forall P, ~~ P -> P.
+
+Lemma drinker : exists p:Person, ~ Mortal p -> forall q:Person, ~ (Mortal q).
+Proof.
+  apply EM.
+  intro.
+  apply H.
+  exists Socrate.
+  intros.
+  intro.
+  apply H.
+  exists q.
+  intro.
+  contradiction.
+Qed.
+
+(* 3.3 Equality *)
+
+(* Example *)
+
+Goal forall x y : nat, x = S y -> y = pred x.
+Proof.
+  intros x y e.
+  rewrite e. 
+  simpl.
+  reflexivity.
+Qed.
+
+(* Require Import Classical.
+Check NNPP. *)
+
+(* 3.4 Groups *)
+(* Modelization using axioms + equational reasoning using rewrite/reflexivity/symmetry/transivitity *)
+
+Parameter (G:Type).
+Parameter op : G -> G -> G.
+Parameter inv : G -> G.
+Parameter e : G.
+
+Axiom assoc  : forall (a b c : G),  op (op a b)  c = op a  (op b c).
+Axiom id_l : forall (a: G), op a e = a.  
+Axiom id_r : forall (a: G), op e a = a.
+
+Axiom inv_r : forall (a:G), op a (inv a) = e.
+Axiom inv_l : forall (a:G), op (inv a) a = e.
+
+Lemma group (x y:G) : inv (op x y) = op (inv y) (inv x).
+Proof.
+  transitivity (op (inv y) (op (inv x) (op (op x y) (inv (op x y))))).
+  - rewrite assoc.
+    rewrite <- assoc with (a:=inv x) (b:=x).
+    rewrite inv_l.
+    rewrite id_r.
+    rewrite <- assoc.
+    rewrite inv_l.
+    rewrite id_r.
+    reflexivity.
+  
+  - rewrite inv_r.
+    rewrite id_l.
+    reflexivity.
+Qed.
+
